@prefix : <https://w3id.org/polifonia/ontology/tunes/> .
@prefix mm: <https://w3id.org/polifonia/ontology/music-meta/> .
@prefix owl: <http://www.w3.org/2002/07/owl#> .
@prefix rdf: <http://www.w3.org/1999/02/22-rdf-syntax-ns#> .
@prefix xml: <http://www.w3.org/XML/1998/namespace> .
@prefix xsd: <http://www.w3.org/2001/XMLSchema#> .
@prefix core: <https://w3id.org/polifonia/ontology/core/> .
@prefix rdfs: <http://www.w3.org/2000/01/rdf-schema#> .
@base <https://w3id.org/polifonia/ontology/tunes/> .

<https://w3id.org/polifonia/ontology/tunes/> rdf:type owl:Ontology ;
                                              owl:versionIRI <https://w3id.org/polifonia/ontology/tunes/1.0/> ;
                                              owl:imports <https://w3id.org/polifonia/ontology/music-meta/1.0/> ;
                                              <http://purl.org/dc/elements/1.1/creator> "Andrea Poltronieri (UniBo)"@en ,
                                                                                        "Jacopo de Berardinis (KCL)"@en ,
                                                                                        "Nicolas Lazzari (UniBo)"@en ,
                                                                                        "Valenitna Carriero (UniBo)"@en ;
                                              <http://purl.org/dc/elements/1.1/license> <https://creativecommons.org/licenses/by-sa/4.0/> ;
                                              rdfs:comment "The Tunes module extends and specialises Music Meta for folk music. The main novelty consists in grouping and describing tunes into “tune families” depending on their melodic similarity (an association requiring rich provenance description of the musicological analysis on the source); which also extends to lyrics families."@en ;
                                              rdfs:label "Tunes Ontology"@en .

#################################################################
#    Annotation properties
#################################################################

###  http://purl.org/dc/elements/1.1/creator
<http://purl.org/dc/elements/1.1/creator> rdf:type owl:AnnotationProperty .


###  http://purl.org/dc/elements/1.1/license
<http://purl.org/dc/elements/1.1/license> rdf:type owl:AnnotationProperty .


#################################################################
#    Object Properties
#################################################################

###  https://w3id.org/polifonia/ontology/core/hasSource
core:hasSource rdfs:domain :Tune ;
               rdfs:range core:Source .


###  https://w3id.org/polifonia/ontology/core/isInvolvedIn
core:isInvolvedIn rdfs:domain mm:Lyrics ,
                              mm:MusicEntity .


#################################################################
#    Classes
#################################################################

###  https://w3id.org/polifonia/ontology/tunes/LyricsFamily
:LyricsFamily rdf:type owl:Class ;
              rdfs:subClassOf core:Collection ;
              rdfs:comment "A collection of lyrics intended as any container for lyrics that share one or more common properties."@en ;
              rdfs:label "Lyrics Family"@en .


###  https://w3id.org/polifonia/ontology/tunes/Tune
:Tune rdf:type owl:Class ;
      rdfs:subClassOf mm:MusicEntity ,
                      [ rdf:type owl:Restriction ;
                        owl:onProperty core:hasSource ;
                        owl:allValuesFrom core:Source
                      ] ;
      rdfs:label "Tune"@en .


###  https://w3id.org/polifonia/ontology/tunes/TuneFamily
:TuneFamily rdf:type owl:Class ;
            rdfs:subClassOf core:Collection ;
            rdfs:comment "A collection of tunes intended as any container for tunes that share one or more common properties."@en ;
            rdfs:label "Tune Family"@en .


###  Generated by the OWL API (version 4.5.9.2019-02-01T07:24:44Z) https://github.com/owlcs/owlapi
